src/opt/Composition.v
@@ -15,8 +15,191 @@ Require Import Simulation.
 
 Set Implicit Arguments.
 
-(* TODO *)
-Lemma sim_compose:
-  True.
+Section Compose.
+  Variable (ths1 ths2:Threads.t).
+  Hypothesis (DISJOINT: Threads.disjoint ths1 ths2).
+
+  Lemma compose_comm:
+    Threads.compose ths1 ths2 = Threads.compose ths2 ths1.
+  Proof.
+    apply IdentMap.eq_leibniz. ii.
+    rewrite ? Threads.compose_spec.
+    unfold Threads.compose_option.
+    destruct (IdentMap.find y ths1) eqn:SRC,
+             (IdentMap.find y ths2) eqn:TGT; auto.
+    exfalso. inv DISJOINT. eapply THREAD; eauto.
+  Qed.
+
+  Lemma compose_forall P:
+    (forall tid lang th (TH: IdentMap.find tid (Threads.compose ths1 ths2) = Some (existT _ lang th)),
+        (P tid lang th):Prop) <->
+    (forall tid lang th (TH: IdentMap.find tid ths1 = Some (existT _ lang th)),
+        (P tid lang th):Prop) /\
+    (forall tid lang th (TH: IdentMap.find tid ths2 = Some (existT _ lang th)),
+        (P tid lang th):Prop).
+  Proof.
+    econs; i.
+    - splits.
+      + intros tid lang th TH.
+        eapply H; eauto.
+        rewrite Threads.compose_spec. rewrite TH. auto.
+      + rewrite compose_comm in H; auto.
+        intros tid lang th TH.
+        eapply H; eauto.
+        rewrite Threads.compose_spec. rewrite TH. auto.
+    - des.
+      rewrite Threads.compose_spec in TH.
+      unfold Threads.compose_option in TH.
+      destruct (IdentMap.find tid ths1) eqn:SRC; inv TH.
+      + eapply H; eauto.
+      + eapply H0; eauto.
+  Qed.
+
+  Lemma compose_is_terminal:
+    Threads.is_terminal (Threads.compose ths1 ths2) <->
+    Threads.is_terminal ths1 /\ Threads.is_terminal ths2.
+  Proof. apply compose_forall. Qed.
+
+  Lemma compose_le mem:
+    Threads.le (Threads.compose ths1 ths2) mem <->
+    Threads.le ths1 mem /\ Threads.le ths2 mem.
+  Proof. apply compose_forall. Qed.
+
+  Lemma compose_consistent mem:
+    Configuration.consistent (Configuration.mk (Threads.compose ths1 ths2) mem) <->
+    Configuration.consistent (Configuration.mk ths1 mem) /\
+    Configuration.consistent (Configuration.mk ths2 mem).
+  Proof. apply compose_forall. Qed.
+
+  Lemma compose_step
+        e mem ths' mem'
+        (STEP: Configuration.step
+                 e
+                 (Configuration.mk (Threads.compose ths1 ths2) mem)
+                 (Configuration.mk ths' mem')):
+    (exists ths1',
+        <<NEXT: ths' = Threads.compose ths1' ths2>> /\
+        <<STEP: Configuration.step
+                  e
+                  (Configuration.mk ths1 mem)
+                  (Configuration.mk ths1' mem')>>) \/
+    (exists ths2',
+        <<NEXT: ths' = Threads.compose ths1 ths2'>> /\
+        <<STEP: Configuration.step
+                  e
+                  (Configuration.mk ths2 mem)
+                  (Configuration.mk ths2' mem')>>).
+  Proof.
+  Admitted.
+
+  Lemma compose_step1
+        e mem ths1' mem'
+        (STEP: Configuration.step
+                 e
+                 (Configuration.mk ths1 mem)
+                 (Configuration.mk ths1' mem')):
+    <<DISJOINT: Threads.disjoint ths1' ths2>> /\
+    <<STEP: Configuration.step
+              e
+              (Configuration.mk (Threads.compose ths1 ths2) mem)
+              (Configuration.mk (Threads.compose ths1' ths2) mem')>>.
+  Proof.
+  Admitted.
+End Compose.
+
+Lemma disjoint_comm
+      ths1 ths2
+      (DISJOINT: Threads.disjoint ths1 ths2):
+  Threads.disjoint ths2 ths1.
 Proof.
+  inv DISJOINT. econs; i.
+  - eapply THREAD; eauto.
+  - apply Memory.disjoint_comm. eapply MEMORY; eauto.
+Qed.
+
+Lemma compose_step2
+      ths1 ths2
+      (DISJOINT: Threads.disjoint ths1 ths2)
+      e mem ths2' mem'
+      (STEP: Configuration.step
+               e
+               (Configuration.mk ths2 mem)
+               (Configuration.mk ths2' mem')):
+  <<DISJOINT: Threads.disjoint ths1 ths2'>> /\
+  <<STEP: Configuration.step
+            e
+            (Configuration.mk (Threads.compose ths1 ths2) mem)
+            (Configuration.mk (Threads.compose ths1 ths2') mem')>>.
+Proof.
+  exploit compose_step1; [|apply STEP|].
+  { apply disjoint_comm. eauto. }
+  i. des. splits.
+  { apply disjoint_comm. eauto. }
+  rewrite (@compose_comm ths1 ths2); auto.
+  rewrite (@compose_comm ths1 ths2'); auto.
+  apply disjoint_comm. eauto.
+Qed.
+
+Lemma sim_compose
+      ths1_src ths2_src mem_k_src
+      ths1_tgt ths2_tgt mem_k_tgt
+      (DISJOINT_SRC: Threads.disjoint ths1_src ths2_src)
+      (DISJOINT_TGT: Threads.disjoint ths1_tgt ths2_tgt)
+      (SIM1: sim ths1_src mem_k_src ths1_tgt mem_k_tgt)
+      (SIM2: sim ths2_src mem_k_src ths2_tgt mem_k_tgt):
+  sim (Threads.compose ths1_src ths2_src) mem_k_src
+      (Threads.compose ths1_tgt ths2_tgt) mem_k_tgt.
+Proof.
+  revert
+    ths1_src ths2_src mem_k_src
+    ths1_tgt ths2_tgt mem_k_tgt
+    DISJOINT_SRC DISJOINT_TGT
+    SIM1 SIM2.
+  pcofix CIH. i. pfold. ii.
+  apply compose_le in LOCAL_SRC; auto.
+  apply compose_le in LOCAL_TGT; auto.
+  splits.
+  - i. des.
+    punfold SIM1. exploit SIM1; eauto. i. des.
+    apply compose_is_terminal in TERMINAL_TGT; auto. des.
+    exploit TERMINAL; eauto. i. des.
+    punfold SIM2. exploit SIM2; eauto.
+    { admit. (* other threads' le *) }
+    { admit. (* future *) }
+    i. des.
+    exploit TERMINAL0; eauto. i. des.
+    eexists _, _. splits; [|eauto|].
+    + admit. (* steps *)
+    + apply compose_is_terminal.
+      * admit. (* disjoint *)
+      * split. apply TERMINAL_SRC. apply TERMINAL_SRC0.
+  - i. apply compose_consistent in CONSISTENT_TGT; auto. des.
+    apply compose_consistent; auto. splits.
+    + punfold SIM1. exploit SIM1; eauto. i. des.
+      apply CONSISTENT. auto.
+    + punfold SIM2. exploit SIM2; eauto. i. des.
+      apply CONSISTENT. auto.
+  - i. apply compose_step in STEP_TGT. des; subst.
+    + punfold SIM1. exploit SIM1; eauto. i. des.
+      exploit STEP0; eauto. i. des; [|done].
+      eexists _, _, _, _. splits.
+      * admit. (* steps *)
+      * apply compose_step1; [|eauto].
+        admit. (* disjoint *)
+      * eauto.
+      * right. apply CIH; [| |eauto|].
+        { admit. (* disjoint *) }
+        { admit. (* disjoint *) }
+        { admit. (* sim future *) }
+    + punfold SIM2. exploit SIM2; eauto. i. des.
+      exploit STEP0; eauto. i. des; [|done].
+      eexists _, _, _, _. splits.
+      * admit. (* steps *)
+      * apply compose_step2; [|eauto].
+        admit. (* disjoint *)
+      * eauto.
+      * right. apply CIH; [| |eauto|].
+        { admit. (* disjoint *) }
+        { admit. (* disjoint *) }
+        { admit. (* sim future *) }
 Admitted.
